Update AThread.v

src/attachable/AThread.v
@@ -18,79 +18,42 @@ Require Import Cell.
 Require Import Memory.
 Require Import TView.
 Require Import Local.
+Require Import Thread.
+
+Require Import AMemory.
+Require Import ATView.
+Require Import ALocal.
 
 Set Implicit Arguments.
 
 
-Inductive tau T (step: forall (e:ThreadEvent.t) (e1 e2:T), Prop) (e1 e2:T): Prop :=
-| tau_intro
-    e
-    (TSTEP: step e e1 e2)
-    (EVENT: ThreadEvent.get_machine_event e = MachineEvent.silent)
-.
-Hint Constructors tau.
-
-Inductive union E T (step: forall (e:E) (e1 e2:T), Prop) (e1 e2:T): Prop :=
-| union_intro
-    e
-    (USTEP: step e e1 e2)
-.
-Hint Constructors union.
-
-Lemma tau_mon T (step1 step2: forall (e:ThreadEvent.t) (e1 e2:T), Prop)
-      (STEP: step1 <3= step2):
-  tau step1 <2= tau step2.
-Proof.
-  i. inv PR. econs; eauto.
-Qed.
-
-Lemma union_mon E T (step1 step2: forall (e:E) (e1 e2:T), Prop)
-      (STEP: step1 <3= step2):
-  union step1 <2= union step2.
-Proof.
-  i. inv PR. econs; eauto.
-Qed.
-
-Lemma tau_union: tau <4= (@union ThreadEvent.t).
-Proof.
-  ii. inv PR. econs. eauto.
-Qed.
-
-
-Module Thread.
-  Section Thread.
+Module AThread.
+  Section AThread.
     Variable (lang:language).
 
-    Structure t := mk {
-      state: lang.(Language.state);
-      local: Local.t;
-      sc: TimeMap.t;
-      memory: Memory.t;
-    }.
-
-    Inductive promise_step (pf:bool): forall (e:ThreadEvent.t) (e1 e2:t), Prop :=
+    Inductive promise_step (pf:bool): forall (e:ThreadEvent.t) (e1 e2:Thread.t lang), Prop :=
     | promise_step_intro
         st lc1 sc1 mem1
         loc from to msg kind
         lc2 mem2
-        (LOCAL: Local.promise_step lc1 mem1 loc from to msg lc2 mem2 kind)
+        (LOCAL: ALocal.promise_step lc1 mem1 loc from to msg lc2 mem2 kind)
         (PF: pf = orb (andb (Memory.op_kind_is_lower_full kind) (Message.is_released_none msg))
                       (Memory.op_kind_is_cancel kind)):
-        promise_step pf (ThreadEvent.promise loc from to msg kind) (mk st lc1 sc1 mem1) (mk st lc2 sc1 mem2)
+        promise_step pf (ThreadEvent.promise loc from to msg kind) (Thread.mk lang st lc1 sc1 mem1) (Thread.mk lang st lc2 sc1 mem2)
     .
 
     (* NOTE: Syscalls act like a SC fence. *)
-    Inductive program_step (e:ThreadEvent.t): forall (e1 e2:t), Prop :=
+    Inductive program_step (e:ThreadEvent.t): forall (e1 e2:Thread.t lang), Prop :=
     | program_step_intro
         st1 lc1 sc1 mem1
         st2 lc2 sc2 mem2
         (STATE: lang.(Language.step) (ThreadEvent.get_program_event e) st1 st2)
-        (LOCAL: Local.program_step e lc1 sc1 mem1 lc2 sc2 mem2):
-        program_step e (mk st1 lc1 sc1 mem1) (mk st2 lc2 sc2 mem2)
+        (LOCAL: ALocal.program_step e lc1 sc1 mem1 lc2 sc2 mem2):
+        program_step e (Thread.mk lang st1 lc1 sc1 mem1) (Thread.mk lang st2 lc2 sc2 mem2)
     .
     Hint Constructors program_step.
 
-    Inductive step: forall (pf:bool) (e:ThreadEvent.t) (e1 e2:t), Prop :=
+    Inductive step: forall (pf:bool) (e:ThreadEvent.t) (e1 e2:Thread.t lang), Prop :=
     | step_promise
         pf e e1 e2
         (STEP: promise_step pf e e1 e2):
@@ -102,7 +65,7 @@ Module Thread.
     .
     Hint Constructors step.
 
-    Inductive step_allpf (e:ThreadEvent.t) (e1 e2:t): Prop :=
+    Inductive step_allpf (e:ThreadEvent.t) (e1 e2:Thread.t lang): Prop :=
     | step_nopf_intro
         pf
         (STEP: step pf e e1 e2)
@@ -123,7 +86,7 @@ Module Thread.
     Definition all_step := union step_allpf.
     Hint Unfold all_step.
 
-    Inductive opt_step: forall (e:ThreadEvent.t) (e1 e2:t), Prop :=
+    Inductive opt_step: forall (e:ThreadEvent.t) (e1 e2:Thread.t lang), Prop :=
     | step_none
         e:
         opt_step ThreadEvent.silent e e
@@ -134,20 +97,20 @@ Module Thread.
     .
     Hint Constructors opt_step.
 
-    Definition steps_failure (e1: t): Prop :=
+    Definition steps_failure (e1: Thread.t lang): Prop :=
       exists e2 e3,
         <<STEPS: rtc tau_step e1 e2>> /\
         <<FAILURE: step true ThreadEvent.failure e2 e3>>.
     Hint Unfold steps_failure.
 
-    Definition consistent (e:t): Prop :=
+    Definition consistent (e:Thread.t lang): Prop :=
       forall mem1 sc1
-        (CAP: Memory.cap e.(local).(Local.promises) e.(memory) mem1)
+        (CAP: Memory.cap e.(Thread.local).(Local.promises) e.(Thread.memory) mem1)
         (SC_MAX: Memory.max_full_timemap mem1 sc1),
-        <<FAILURE: steps_failure (mk e.(state) e.(local) sc1 mem1)>> \/
+        <<FAILURE: steps_failure (Thread.mk lang e.(Thread.state) e.(Thread.local) sc1 mem1)>> \/
         exists e2,
-          <<STEPS: rtc tau_step (mk e.(state) e.(local) sc1 mem1) e2>> /\
-          <<PROMISES: e2.(local).(Local.promises) = Memory.bot>>.
+          <<STEPS: rtc tau_step (Thread.mk lang e.(Thread.state) e.(Thread.local) sc1 mem1) e2>> /\
+          <<PROMISES: e2.(Thread.local).(Local.promises) = Memory.bot>>.
 
 
     (* step_future *)
@@ -155,87 +118,67 @@ Module Thread.
     Lemma promise_step_future
           pf e e1 e2
           (STEP: promise_step pf e e1 e2)
-          (WF1: Local.wf e1.(local) e1.(memory))
-          (SC1: Memory.closed_timemap e1.(sc) e1.(memory))
-          (CLOSED1: Memory.closed e1.(memory)):
-      <<WF2: Local.wf e2.(local) e2.(memory)>> /\
-      <<SC2: Memory.closed_timemap e2.(sc) e2.(memory)>> /\
-      <<CLOSED2: Memory.closed e2.(memory)>> /\
+          (WF1: Local.wf e1.(Thread.local) e1.(Thread.memory))
+          (SC1: Memory.closed_timemap e1.(Thread.sc) e1.(Thread.memory))
+          (CLOSED1: Memory.closed e1.(Thread.memory)):
+      <<WF2: Local.wf e2.(Thread.local) e2.(Thread.memory)>> /\
+      <<SC2: Memory.closed_timemap e2.(Thread.sc) e2.(Thread.memory)>> /\
+      <<CLOSED2: Memory.closed e2.(Thread.memory)>> /\
       <<TVIEW_FUTURE: TView.le e1.(Thread.local).(Local.tview) e2.(Thread.local).(Local.tview)>> /\
-      <<SC_FUTURE: TimeMap.le e1.(sc) e2.(sc)>> /\
-      <<MEM_FUTURE: Memory.future e1.(memory) e2.(memory)>>.
+      <<SC_FUTURE: TimeMap.le e1.(Thread.sc) e2.(Thread.sc)>> /\
+      <<MEM_FUTURE: Memory.future e1.(Thread.memory) e2.(Thread.memory)>>.
     Proof.
       inv STEP. ss.
-      exploit Local.promise_step_future; eauto. i. des.
+      exploit ALocal.promise_step_future; eauto. i. des.
       splits; eauto. refl.
     Qed.
 
     Lemma program_step_future
           e e1 e2
           (STEP: program_step e e1 e2)
-          (WF1: Local.wf e1.(local) e1.(memory))
-          (SC1: Memory.closed_timemap e1.(sc) e1.(memory))
-          (CLOSED1: Memory.closed e1.(memory)):
-      <<WF2: Local.wf e2.(local) e2.(memory)>> /\
-      <<SC2: Memory.closed_timemap e2.(sc) e2.(memory)>> /\
-      <<CLOSED2: Memory.closed e2.(memory)>> /\
+          (WF1: Local.wf e1.(Thread.local) e1.(Thread.memory))
+          (SC1: Memory.closed_timemap e1.(Thread.sc) e1.(Thread.memory))
+          (CLOSED1: Memory.closed e1.(Thread.memory)):
+      <<WF2: Local.wf e2.(Thread.local) e2.(Thread.memory)>> /\
+      <<SC2: Memory.closed_timemap e2.(Thread.sc) e2.(Thread.memory)>> /\
+      <<CLOSED2: Memory.closed e2.(Thread.memory)>> /\
       <<TVIEW_FUTURE: TView.le e1.(Thread.local).(Local.tview) e2.(Thread.local).(Local.tview)>> /\
-      <<SC_FUTURE: TimeMap.le e1.(sc) e2.(sc)>> /\
-      <<MEM_FUTURE: Memory.future e1.(memory) e2.(memory)>>.
+      <<SC_FUTURE: TimeMap.le e1.(Thread.sc) e2.(Thread.sc)>> /\
+      <<MEM_FUTURE: Memory.future e1.(Thread.memory) e2.(Thread.memory)>>.
     Proof.
-      inv STEP. ss. eapply Local.program_step_future; eauto.
+      inv STEP. ss. eapply ALocal.program_step_future; eauto.
     Qed.
 
     Lemma step_future
           pf e e1 e2
           (STEP: step pf e e1 e2)
-          (WF1: Local.wf e1.(local) e1.(memory))
-          (SC1: Memory.closed_timemap e1.(sc) e1.(memory))
-          (CLOSED1: Memory.closed e1.(memory)):
-      <<WF2: Local.wf e2.(local) e2.(memory)>> /\
-      <<SC2: Memory.closed_timemap e2.(sc) e2.(memory)>> /\
-      <<CLOSED2: Memory.closed e2.(memory)>> /\
+          (WF1: Local.wf e1.(Thread.local) e1.(Thread.memory))
+          (SC1: Memory.closed_timemap e1.(Thread.sc) e1.(Thread.memory))
+          (CLOSED1: Memory.closed e1.(Thread.memory)):
+      <<WF2: Local.wf e2.(Thread.local) e2.(Thread.memory)>> /\
+      <<SC2: Memory.closed_timemap e2.(Thread.sc) e2.(Thread.memory)>> /\
+      <<CLOSED2: Memory.closed e2.(Thread.memory)>> /\
       <<TVIEW_FUTURE: TView.le e1.(Thread.local).(Local.tview) e2.(Thread.local).(Local.tview)>> /\
-      <<SC_FUTURE: TimeMap.le e1.(sc) e2.(sc)>> /\
-      <<MEM_FUTURE: Memory.future e1.(memory) e2.(memory)>>.
+      <<SC_FUTURE: TimeMap.le e1.(Thread.sc) e2.(Thread.sc)>> /\
+      <<MEM_FUTURE: Memory.future e1.(Thread.memory) e2.(Thread.memory)>>.
     Proof.
       inv STEP.
       - eapply promise_step_future; eauto.
       - eapply program_step_future; eauto.
     Qed.
 
-    (* TODO: unused *)
-    Lemma step_nonpf_future
-          e e1 e2
-          (STEP: step false e e1 e2)
-          (WF1: Local.wf e1.(local) e1.(memory))
-          (SC1: Memory.closed_timemap e1.(sc) e1.(memory))
-          (CLOSED1: Memory.closed e1.(memory)):
-      <<WF2: Local.wf e2.(local) e2.(memory)>> /\
-      <<SC2: Memory.closed_timemap e2.(sc) e2.(memory)>> /\
-      <<CLOSED2: Memory.closed e2.(memory)>> /\
-      <<TVIEW_FUTURE: TView.le e1.(local).(Local.tview) e2.(local).(Local.tview)>> /\
-      <<SC_FUTURE: TimeMap.le e1.(sc) e2.(sc)>> /\
-      <<MEM_FUTURE: Memory.future e1.(memory) e2.(memory)>> /\
-      <<STATE: e1.(state) = e2.(state)>>.
-    Proof.
-      inv STEP. inv STEP0. ss.
-      exploit Local.promise_step_future; eauto. i. des.
-      esplits; ss. refl.
-    Qed.
-
     Lemma opt_step_future
           e e1 e2
           (STEP: opt_step e e1 e2)
-          (WF1: Local.wf e1.(local) e1.(memory))
-          (SC1: Memory.closed_timemap e1.(sc) e1.(memory))
-          (CLOSED1: Memory.closed e1.(memory)):
-      <<WF2: Local.wf e2.(local) e2.(memory)>> /\
-      <<SC2: Memory.closed_timemap e2.(sc) e2.(memory)>> /\
-      <<CLOSED2: Memory.closed e2.(memory)>> /\
+          (WF1: Local.wf e1.(Thread.local) e1.(Thread.memory))
+          (SC1: Memory.closed_timemap e1.(Thread.sc) e1.(Thread.memory))
+          (CLOSED1: Memory.closed e1.(Thread.memory)):
+      <<WF2: Local.wf e2.(Thread.local) e2.(Thread.memory)>> /\
+      <<SC2: Memory.closed_timemap e2.(Thread.sc) e2.(Thread.memory)>> /\
+      <<CLOSED2: Memory.closed e2.(Thread.memory)>> /\
       <<TVIEW_FUTURE: TView.le e1.(Thread.local).(Local.tview) e2.(Thread.local).(Local.tview)>> /\
-      <<SC_FUTURE: TimeMap.le e1.(sc) e2.(sc)>> /\
-      <<MEM_FUTURE: Memory.future e1.(memory) e2.(memory)>>.
+      <<SC_FUTURE: TimeMap.le e1.(Thread.sc) e2.(Thread.sc)>> /\
+      <<MEM_FUTURE: Memory.future e1.(Thread.memory) e2.(Thread.memory)>>.
     Proof.
       inv STEP.
       - esplits; eauto; refl.
@@ -245,15 +188,15 @@ Module Thread.
     Lemma rtc_all_step_future
           e1 e2
           (STEP: rtc all_step e1 e2)
-          (WF1: Local.wf e1.(local) e1.(memory))
-          (SC1: Memory.closed_timemap e1.(sc) e1.(memory))
-          (CLOSED1: Memory.closed e1.(memory)):
-      <<WF2: Local.wf e2.(local) e2.(memory)>> /\
-      <<SC2: Memory.closed_timemap e2.(sc) e2.(memory)>> /\
-      <<CLOSED2: Memory.closed e2.(memory)>> /\
+          (WF1: Local.wf e1.(Thread.local) e1.(Thread.memory))
+          (SC1: Memory.closed_timemap e1.(Thread.sc) e1.(Thread.memory))
+          (CLOSED1: Memory.closed e1.(Thread.memory)):
+      <<WF2: Local.wf e2.(Thread.local) e2.(Thread.memory)>> /\
+      <<SC2: Memory.closed_timemap e2.(Thread.sc) e2.(Thread.memory)>> /\
+      <<CLOSED2: Memory.closed e2.(Thread.memory)>> /\
       <<TVIEW_FUTURE: TView.le e1.(Thread.local).(Local.tview) e2.(Thread.local).(Local.tview)>> /\
-      <<SC_FUTURE: TimeMap.le e1.(sc) e2.(sc)>> /\
-      <<MEM_FUTURE: Memory.future e1.(memory) e2.(memory)>>.
+      <<SC_FUTURE: TimeMap.le e1.(Thread.sc) e2.(Thread.sc)>> /\
+      <<MEM_FUTURE: Memory.future e1.(Thread.memory) e2.(Thread.memory)>>.
     Proof.
       revert WF1. induction STEP.
       - i. splits; ss; refl.
@@ -266,68 +209,46 @@ Module Thread.
     Lemma rtc_tau_step_future
           e1 e2
           (STEP: rtc tau_step e1 e2)
-          (WF1: Local.wf e1.(local) e1.(memory))
-          (SC1: Memory.closed_timemap e1.(sc) e1.(memory))
-          (CLOSED1: Memory.closed e1.(memory)):
-      <<WF2: Local.wf e2.(local) e2.(memory)>> /\
-      <<SC2: Memory.closed_timemap e2.(sc) e2.(memory)>> /\
-      <<CLOSED2: Memory.closed e2.(memory)>> /\
+          (WF1: Local.wf e1.(Thread.local) e1.(Thread.memory))
+          (SC1: Memory.closed_timemap e1.(Thread.sc) e1.(Thread.memory))
+          (CLOSED1: Memory.closed e1.(Thread.memory)):
+      <<WF2: Local.wf e2.(Thread.local) e2.(Thread.memory)>> /\
+      <<SC2: Memory.closed_timemap e2.(Thread.sc) e2.(Thread.memory)>> /\
+      <<CLOSED2: Memory.closed e2.(Thread.memory)>> /\
       <<TVIEW_FUTURE: TView.le e1.(Thread.local).(Local.tview) e2.(Thread.local).(Local.tview)>> /\
-      <<SC_FUTURE: TimeMap.le e1.(sc) e2.(sc)>> /\
-      <<MEM_FUTURE: Memory.future e1.(memory) e2.(memory)>>.
+      <<SC_FUTURE: TimeMap.le e1.(Thread.sc) e2.(Thread.sc)>> /\
+      <<MEM_FUTURE: Memory.future e1.(Thread.memory) e2.(Thread.memory)>>.
     Proof.
       apply rtc_all_step_future; auto.
       eapply rtc_implies; [|eauto].
       apply tau_union.
     Qed.
 
-    (* TODO: unused *)
-    Lemma rtc_step_nonpf_future
-          e1 e2
-          (STEP: rtc (union (step false)) e1 e2)
-          (WF1: Local.wf e1.(local) e1.(memory))
-          (SC1: Memory.closed_timemap e1.(sc) e1.(memory))
-          (CLOSED1: Memory.closed e1.(memory)):
-      <<WF2: Local.wf e2.(local) e2.(memory)>> /\
-      <<SC2: Memory.closed_timemap e2.(sc) e2.(memory)>> /\
-      <<CLOSED2: Memory.closed e2.(memory)>> /\
-      <<TVIEW_FUTURE: TView.le e1.(local).(Local.tview) e2.(local).(Local.tview)>> /\
-      <<SC_FUTURE: TimeMap.le e1.(sc) e2.(sc)>> /\
-      <<MEM_FUTURE: Memory.future e1.(memory) e2.(memory)>> /\
-      <<STATE: e1.(state) = e2.(state)>>.
-    Proof.
-      revert WF1. induction STEP.
-      - i. splits; ss; refl.
-      - inv H. i. exploit step_nonpf_future; eauto. i. des.
-        exploit IHSTEP; eauto. i. des.
-        splits; ss; etrans; eauto.
-    Qed.
-
     Lemma promise_step_inhabited
           pf e e1 e2
           (STEP: promise_step pf e e1 e2)
-          (INHABITED1: Memory.inhabited e1.(memory)):
-      <<INHABITED2: Memory.inhabited e2.(memory)>>.
+          (INHABITED1: Memory.inhabited e1.(Thread.memory)):
+      <<INHABITED2: Memory.inhabited e2.(Thread.memory)>>.
     Proof.
       inv STEP. ss.
-      eapply Local.promise_step_inhabited; eauto.
+      eapply ALocal.promise_step_inhabited; eauto.
     Qed.
 
     Lemma program_step_inhabited
           e e1 e2
           (STEP: program_step e e1 e2)
-          (INHABITED1: Memory.inhabited e1.(memory)):
-      <<INHABITED2: Memory.inhabited e2.(memory)>>.
+          (INHABITED1: Memory.inhabited e1.(Thread.memory)):
+      <<INHABITED2: Memory.inhabited e2.(Thread.memory)>>.
     Proof.
       inv STEP. ss.
-      eapply Local.program_step_inhabited; eauto.
+      eapply ALocal.program_step_inhabited; eauto.
     Qed.
 
     Lemma step_inhabited
           pf e e1 e2
           (STEP: step pf e e1 e2)
-          (INHABITED1: Memory.inhabited e1.(memory)):
-      <<INHABITED2: Memory.inhabited e2.(memory)>>.
+          (INHABITED1: Memory.inhabited e1.(Thread.memory)):
+      <<INHABITED2: Memory.inhabited e2.(Thread.memory)>>.
     Proof.
       inv STEP.
       - eapply promise_step_inhabited; eauto.
@@ -340,43 +261,43 @@ Module Thread.
     Lemma promise_step_disjoint
           pf e e1 e2 lc
           (STEP: promise_step pf e e1 e2)
-          (WF1: Local.wf e1.(local) e1.(memory))
-          (SC1: Memory.closed_timemap e1.(sc) e1.(memory))
-          (CLOSED1: Memory.closed e1.(memory))
-          (DISJOINT1: Local.disjoint e1.(local) lc)
-          (WF: Local.wf lc e1.(memory)):
-      <<DISJOINT2: Local.disjoint e2.(local) lc>> /\
-      <<WF: Local.wf lc e2.(memory)>>.
+          (WF1: Local.wf e1.(Thread.local) e1.(Thread.memory))
+          (SC1: Memory.closed_timemap e1.(Thread.sc) e1.(Thread.memory))
+          (CLOSED1: Memory.closed e1.(Thread.memory))
+          (DISJOINT1: Local.disjoint e1.(Thread.local) lc)
+          (WF: Local.wf lc e1.(Thread.memory)):
+      <<DISJOINT2: Local.disjoint e2.(Thread.local) lc>> /\
+      <<WF: Local.wf lc e2.(Thread.memory)>>.
     Proof.
       inv STEP.
-      exploit Local.promise_step_future; eauto. i. des.
-      exploit Local.promise_step_disjoint; eauto.
+      exploit ALocal.promise_step_future; eauto. i. des.
+      exploit ALocal.promise_step_disjoint; eauto.
     Qed.
 
     Lemma program_step_disjoint
           e e1 e2 lc
           (STEP: program_step e e1 e2)
-          (WF1: Local.wf e1.(local) e1.(memory))
-          (SC1: Memory.closed_timemap e1.(sc) e1.(memory))
-          (CLOSED1: Memory.closed e1.(memory))
-          (DISJOINT1: Local.disjoint e1.(local) lc)
-          (WF: Local.wf lc e1.(memory)):
-      <<DISJOINT2: Local.disjoint e2.(local) lc>> /\
-      <<WF: Local.wf lc e2.(memory)>>.
+          (WF1: Local.wf e1.(Thread.local) e1.(Thread.memory))
+          (SC1: Memory.closed_timemap e1.(Thread.sc) e1.(Thread.memory))
+          (CLOSED1: Memory.closed e1.(Thread.memory))
+          (DISJOINT1: Local.disjoint e1.(Thread.local) lc)
+          (WF: Local.wf lc e1.(Thread.memory)):
+      <<DISJOINT2: Local.disjoint e2.(Thread.local) lc>> /\
+      <<WF: Local.wf lc e2.(Thread.memory)>>.
     Proof.
-      inv STEP. ss. eapply Local.program_step_disjoint; eauto.
+      inv STEP. ss. eapply ALocal.program_step_disjoint; eauto.
     Qed.
 
     Lemma step_disjoint
           pf e e1 e2 lc
           (STEP: step pf e e1 e2)
-          (WF1: Local.wf e1.(local) e1.(memory))
-          (SC1: Memory.closed_timemap e1.(sc) e1.(memory))
-          (CLOSED1: Memory.closed e1.(memory))
-          (DISJOINT1: Local.disjoint e1.(local) lc)
-          (WF: Local.wf lc e1.(memory)):
-      <<DISJOINT2: Local.disjoint e2.(local) lc>> /\
-      <<WF: Local.wf lc e2.(memory)>>.
+          (WF1: Local.wf e1.(Thread.local) e1.(Thread.memory))
+          (SC1: Memory.closed_timemap e1.(Thread.sc) e1.(Thread.memory))
+          (CLOSED1: Memory.closed e1.(Thread.memory))
+          (DISJOINT1: Local.disjoint e1.(Thread.local) lc)
+          (WF: Local.wf lc e1.(Thread.memory)):
+      <<DISJOINT2: Local.disjoint e2.(Thread.local) lc>> /\
+      <<WF: Local.wf lc e2.(Thread.memory)>>.
     Proof.
       inv STEP.
       - eapply promise_step_disjoint; eauto.
@@ -386,13 +307,13 @@ Module Thread.
     Lemma opt_step_disjoint
           e e1 e2 lc
           (STEP: opt_step e e1 e2)
-          (WF1: Local.wf e1.(local) e1.(memory))
-          (SC1: Memory.closed_timemap e1.(sc) e1.(memory))
-          (CLOSED1: Memory.closed e1.(memory))
-          (DISJOINT1: Local.disjoint e1.(local) lc)
-          (WF: Local.wf lc e1.(memory)):
-      <<DISJOINT2: Local.disjoint e2.(local) lc>> /\
-      <<WF: Local.wf lc e2.(memory)>>.
+          (WF1: Local.wf e1.(Thread.local) e1.(Thread.memory))
+          (SC1: Memory.closed_timemap e1.(Thread.sc) e1.(Thread.memory))
+          (CLOSED1: Memory.closed e1.(Thread.memory))
+          (DISJOINT1: Local.disjoint e1.(Thread.local) lc)
+          (WF: Local.wf lc e1.(Thread.memory)):
+      <<DISJOINT2: Local.disjoint e2.(Thread.local) lc>> /\
+      <<WF: Local.wf lc e2.(Thread.memory)>>.
     Proof.
       inv STEP.
       - esplits; eauto.
@@ -402,13 +323,13 @@ Module Thread.
     Lemma rtc_all_step_disjoint
           e1 e2 lc
           (STEP: rtc all_step e1 e2)
-          (WF1: Local.wf e1.(local) e1.(memory))
-          (SC1: Memory.closed_timemap e1.(sc) e1.(memory))
-          (CLOSED1: Memory.closed e1.(memory))
-          (DISJOINT1: Local.disjoint e1.(local) lc)
-          (WF: Local.wf lc e1.(memory)):
-      <<DISJOINT2: Local.disjoint e2.(local) lc>> /\
-      <<WF: Local.wf lc e2.(memory)>>.
+          (WF1: Local.wf e1.(Thread.local) e1.(Thread.memory))
+          (SC1: Memory.closed_timemap e1.(Thread.sc) e1.(Thread.memory))
+          (CLOSED1: Memory.closed e1.(Thread.memory))
+          (DISJOINT1: Local.disjoint e1.(Thread.local) lc)
+          (WF: Local.wf lc e1.(Thread.memory)):
+      <<DISJOINT2: Local.disjoint e2.(Thread.local) lc>> /\
+      <<WF: Local.wf lc e2.(Thread.memory)>>.
     Proof.
       revert WF1 DISJOINT1 WF. induction STEP; eauto. i.
       inv H. inv USTEP.
@@ -420,13 +341,13 @@ Module Thread.
     Lemma rtc_tau_step_disjoint
           e1 e2 lc
           (STEP: rtc tau_step e1 e2)
-          (WF1: Local.wf e1.(local) e1.(memory))
-          (SC1: Memory.closed_timemap e1.(sc) e1.(memory))
-          (CLOSED1: Memory.closed e1.(memory))
-          (DISJOINT1: Local.disjoint e1.(local) lc)
-          (WF: Local.wf lc e1.(memory)):
-      <<DISJOINT2: Local.disjoint e2.(local) lc>> /\
-      <<WF: Local.wf lc e2.(memory)>>.
+          (WF1: Local.wf e1.(Thread.local) e1.(Thread.memory))
+          (SC1: Memory.closed_timemap e1.(Thread.sc) e1.(Thread.memory))
+          (CLOSED1: Memory.closed e1.(Thread.memory))
+          (DISJOINT1: Local.disjoint e1.(Thread.local) lc)
+          (WF: Local.wf lc e1.(Thread.memory)):
+      <<DISJOINT2: Local.disjoint e2.(Thread.local) lc>> /\
+      <<WF: Local.wf lc e2.(Thread.memory)>>.
     Proof.
       eapply rtc_all_step_disjoint; cycle 1; eauto.
       eapply rtc_implies; [|eauto].
@@ -436,29 +357,26 @@ Module Thread.
 
     (* step_no_reserve_except *)
 
-    Definition no_reserve_except (e: t) :=
-      Memory.no_reserve_except e.(local).(Local.promises) e.(memory).
-
     Lemma step_no_reserve_except
           pf e e1 e2
           (STEP: step pf e e1 e2)
-          (WF1: Local.wf e1.(local) e1.(memory))
-          (NORESERVE1: no_reserve_except e1):
-      no_reserve_except e2.
+          (WF1: Local.wf e1.(Thread.local) e1.(Thread.memory))
+          (NORESERVE1: Thread.no_reserve_except e1):
+      Thread.no_reserve_except e2.
     Proof.
       inv STEP; inv STEP0.
-      - eapply Local.promise_step_no_reserve_except; eauto. apply WF1.
-      - eapply Local.program_step_no_reserve_except; eauto. apply WF1.
+      - eapply ALocal.promise_step_no_reserve_except; eauto. apply WF1.
+      - eapply ALocal.program_step_no_reserve_except; eauto. apply WF1.
     Qed.
 
     Lemma rtc_tau_step_no_reserve_except
           e1 e2
           (STEP: rtc tau_step e1 e2)
-          (WF1: Local.wf e1.(local) e1.(memory))
-          (SC1: Memory.closed_timemap e1.(sc) e1.(memory))
-          (CLOSED1: Memory.closed e1.(memory))
-          (NORESERVE1: no_reserve_except e1):
-      no_reserve_except e2.
+          (WF1: Local.wf e1.(Thread.local) e1.(Thread.memory))
+          (SC1: Memory.closed_timemap e1.(Thread.sc) e1.(Thread.memory))
+          (CLOSED1: Memory.closed e1.(Thread.memory))
+          (NORESERVE1: Thread.no_reserve_except e1):
+      Thread.no_reserve_except e2.
     Proof.
       induction STEP; ss; i.
       inv H. inv TSTEP. exploit step_future; eauto. i. des.
@@ -469,17 +387,17 @@ Module Thread.
     Lemma step_bot_no_reserve
           pf e e1 e2
           (STEP: step pf e e1 e2)
-          (WF1: Local.wf e1.(local) e1.(memory))
-          (SC1: Memory.closed_timemap e1.(sc) e1.(memory))
-          (CLOSED1: Memory.closed e1.(memory))
-          (NORESERVE1: Memory.no_reserve e1.(memory))
-          (PROMISES2: e2.(local).(Local.promises) = Memory.bot):
-      Memory.no_reserve e2.(memory).
+          (WF1: Local.wf e1.(Thread.local) e1.(Thread.memory))
+          (SC1: Memory.closed_timemap e1.(Thread.sc) e1.(Thread.memory))
+          (CLOSED1: Memory.closed e1.(Thread.memory))
+          (NORESERVE1: Memory.no_reserve e1.(Thread.memory))
+          (PROMISES2: e2.(Thread.local).(Local.promises) = Memory.bot):
+      Memory.no_reserve e2.(Thread.memory).
     Proof.
       exploit step_future; eauto. i. des.
       hexploit step_no_reserve_except; eauto; i.
       { eapply Memory.no_reserve_no_reserve_except; eauto. }
-      unfold no_reserve_except in *. rewrite PROMISES2 in *.
+      unfold Thread.no_reserve_except in *. rewrite PROMISES2 in *.
       eapply Memory.no_reserve_except_bot_no_reserve; eauto.
       apply CLOSED2.
     Qed.
@@ -487,17 +405,17 @@ Module Thread.
     Lemma rtc_tau_step_bot_no_reserve
           e1 e2
           (STEP: rtc tau_step e1 e2)
-          (WF1: Local.wf e1.(local) e1.(memory))
-          (SC1: Memory.closed_timemap e1.(sc) e1.(memory))
-          (CLOSED1: Memory.closed e1.(memory))
-          (NORESERVE1: Memory.no_reserve e1.(memory))
-          (PROMISES2: e2.(local).(Local.promises) = Memory.bot):
-      Memory.no_reserve e2.(memory).
+          (WF1: Local.wf e1.(Thread.local) e1.(Thread.memory))
+          (SC1: Memory.closed_timemap e1.(Thread.sc) e1.(Thread.memory))
+          (CLOSED1: Memory.closed e1.(Thread.memory))
+          (NORESERVE1: Memory.no_reserve e1.(Thread.memory))
+          (PROMISES2: e2.(Thread.local).(Local.promises) = Memory.bot):
+      Memory.no_reserve e2.(Thread.memory).
     Proof.
       exploit rtc_tau_step_future; eauto. i. des.
       hexploit rtc_tau_step_no_reserve_except; eauto; i.
       { eapply Memory.no_reserve_no_reserve_except; eauto. }
-      unfold no_reserve_except in *. rewrite PROMISES2 in *.
+      unfold Thread.no_reserve_except in *. rewrite PROMISES2 in *.
       eapply Memory.no_reserve_except_bot_no_reserve; eauto.
       apply CLOSED2.
     Qed.
@@ -506,10 +424,10 @@ Module Thread.
     Lemma bot_program_step_bot
           e e1 e2
           (STEP: program_step e e1 e2)
-          (PROMISES: e1.(local).(Local.promises) = Memory.bot):
-      e2.(local).(Local.promises) = Memory.bot.
+          (PROMISES: e1.(Thread.local).(Local.promises) = Memory.bot):
+      e2.(Thread.local).(Local.promises) = Memory.bot.
     Proof.
-      inv STEP. eapply Local.bot_program_step_bot; eauto.
+      inv STEP. eapply ALocal.bot_program_step_bot; eauto.
     Qed.
-  End Thread.
-End Thread.
+  End AThread.
+End AThread.
